BackTrans/Emulate.v
@@ -14,10 +14,12 @@ Require Import LogRel.LemmasPseudoType.
 Require Import LogRel.LR.
 Require Import LogRel.LemmasLR.
 Require Import LogRel.LemmasIntro.
+Require Import LogRel.LemmasInversion.
 Require Import Omega.
 Require Import Db.Lemmas.
 Require Import UVal.UVal.
 Require Utlc.Fix.
+Require Omega.
 
 Fixpoint emulate (n : nat) (t : U.UTm) : S.Tm :=
   match t with
@@ -96,3 +98,186 @@ Proof.
   eauto using toUVals_entry, inUnitDwn_pctx_T, inBoolDwn_pctx_T, inProdDwn_pctx_T, inSumDwn_pctx_T, inArrDwn_pctx_T, caseUnitUp_pctx_T, caseBoolUp_pctx_T, caseProdUp_pctx_T, caseSumUp_pctx_T, caseArrUp_pctx_T, emulate_T, emulate_T', PCtxTyping, caseSumUp_T with typing uval_typing.
 Qed.
 
+Local Ltac crush :=
+  repeat (repeat crushUtlcSyntaxMatchH; 
+          repeat crushStlcSyntaxMatchH; 
+          repeat crushStlcEval; 
+          repeat crushDbSyntaxMatchH;
+          repeat crushDbLemmasMatchH;
+          repeat crushDbLemmasRewriteH;
+          try assumption;
+          crushOfType;
+          trivial;
+          eauto using caseUnit_pctx_ECtx, caseBool_pctx_ECtx, caseProd_pctx_ECtx, caseSum_pctx_ECtx, caseArr_pctx_ECtx, upgrade_value, downgrade_value with typing
+         ).
+
+Lemma compat_emul_abs {n m d p Γ ts tu} :
+  dir_world_prec n m d p →
+  ⟪ Γ p▻ pEmulDV n p ⊩ ts ⟦ d , m ⟧ tu : pEmulDV n p ⟫ →
+  ⟪ Γ ⊩ inArrDwn n (S.abs (UVal n) ts) ⟦ d , m ⟧ U.abs tu : pEmulDV n p ⟫.
+Proof.
+  intros dwp [ty tr].
+  split.
+  - eauto using inArrDwn_T with typing uval_typing.
+  - intros w wn γs γu envrel.
+
+    assert (OfType (ptarr (pEmulDV n p) (pEmulDV n p))
+                   (S.abs (repEmul (pEmulDV n p)) 
+                          (ts [γs↑])) (U.abs (tu [γu↑])))
+      by (pose proof (envrel_implies_WtSub envrel);
+          crush).
+
+    assert (dir_world_prec n w d p) by eauto using dwp_mono.
+
+    rewrite inArrDwn_sub.
+    eapply termrel_inArrDwn; try assumption.
+
+    change (UVal n) with (repEmul (pEmulDV n p)).
+
+    eapply valrel_lambda; crush.
+
+    intros w' vs vu futw valrel.
+
+    fold apTm apUTm.
+    crushUtlcSyntaxMatchH; crushStlcSyntaxMatchH.
+    rewrite ?ap_comp.
+
+    assert (lev w' ≤ m) by (unfold lev in *; Omega.omega).
+
+    eapply tr;
+      eauto using extend_envrel, envrel_mono.
+Qed.
+
+Lemma compat_emul_pabs {n m d p Γ} :
+  dir_world_prec n m d p →
+  ⟪ ⊩ S.pctx_cat (S.pabs (UVal n) S.phole) (inArrDwn_pctx n) ⟦ d , m ⟧ U.pabs U.phole : Γ p▻ pEmulDV n p , pEmulDV n p → Γ , pEmulDV n p ⟫.
+Proof.
+  intros dwp.
+  split.
+  - eauto using inArrDwn_pctx_T with typing uval_typing.
+  - intros ts tu lr.
+    change (S.pctx_app ts (S.pctx_cat (S.pabs (UVal n) S.phole) (inArrDwn_pctx n)))
+    with (inArrDwn n (S.abs (UVal n) ts)).
+    eauto using compat_emul_abs.
+Qed.
+
+Lemma termrel_caseArrUp {d w n p ts₁ tu₁ ts₂ tu₂} :
+  dir_world_prec n w d p →
+  termrel d w (pEmulDV n p) ts₁ tu₁ →
+  (∀ w' : World, w' ≤ w → termrel d w' (pEmulDV n p) ts₂ tu₂) →
+  termrel d w (pEmulDV n p) 
+          (S.app (S.app (S.abs (UVal n) (S.abs (UVal n) (S.app (caseArrUp n (S.var 1)) (S.var 0)))) ts₁) ts₂) (U.app tu₁ tu₂).
+Proof.
+  intros dwp tr₁ tr₂.
+  unfold caseArrUp, caseArrUp_pctx.
+  (* evaluate ts₁ and tu₁ *)
+  eapply (termrel_ectx' tr₁); S.inferContext; U.inferContext; 
+  unfold pctx_cat, U.ECtx; crush.
+
+  (* continuation boilerplate *)
+  intros w' futw vs₁ vu₁ vr₁.
+  destruct (valrel_implies_OfType vr₁) as [[vvs₁ ?] ?].
+  rewrite pctx_cat_app; cbn.
+
+  (* beta-reduce the outer let *)
+  eapply termrel_antired_eval_left.
+  eapply (eval_from_eval₀ (eval_beta vvs₁)); S.inferContext; crush.
+  cbn; crush.
+
+  (* bureaucracy *)
+  fold (caseArr n (S.app (upgrade n 1) (S.var 1))).
+  rewrite caseArr_sub; cbn; crush; rewrite upgrade_sub.
+
+  (* evaluate ts₂ and tu₂ *)
+  specialize (tr₂ w' futw).
+  eapply (termrel_ectx' tr₂); S.inferContext; U.inferContext; 
+  unfold pctx_cat, U.ECtx; crush.
+  
+  (* continuation boilerplate *)
+  intros w'' futw' vs₂ vu₂ vr₂.
+  destruct (valrel_implies_Value vr₂) as [vvs₂ ?].
+  cbn.
+
+  (* beta-reduce the remaining let *)
+  eapply termrel_antired_eval_left.
+  eapply (eval_from_eval₀ (eval_beta vvs₂)); S.inferContext; crush.
+  cbn; crush.
+
+  (* bureaucracy *)
+  fold (caseArr n (S.app (upgrade n 1) (S.var 1))).
+  rewrite ?caseArr_sub; cbn; crush; rewrite ?upgrade_sub.
+  rewrite <- ?ap_liftSub; rewrite -> ?liftSub_wkm; rewrite (apply_wkm_beta1_cancel vs₁ vs₂).
+  
+  (* execute the upgrade *)
+  assert (w'' ≤ w) by Omega.omega.
+  assert (valrel d w'' (pEmulDV n p) vs₁ vu₁) by eauto using valrel_mono.
+  assert (trupg : termrel d w'' (pEmulDV (n + 1) p) (S.app (upgrade n 1) vs₁) vu₁)
+    by (eauto using upgrade_works', dwp_mono).
+  unfold caseArr.
+  eapply (termrel_ectx' trupg); S.inferContext; U.inferContext; cbn; crush.
+
+  (* continuation bureaucracy *)
+  intros w''' futw'' vs₁' vu₁' vr₁'.
+  replace (n + 1) with (S n) in vr₁' by Omega.omega.
+
+  destruct (valrel_implies_Value vr₁').
+  (* case analysis *)
+  eapply invert_valrel_pEmulDV_for_caseUValArr in vr₁'.
+  destruct vr₁' as [(vs₁'' & ? & es & vr₁')|[(? & div)|(neq & div)]]; subst.
+  - (* Correct case *)
+
+    (* caseArr succeeds *)
+    eapply termrel_antired_star_left.
+    fold (caseArr n (inArr n vs₁'')).
+    eapply (evalstar_ctx' es); S.inferContext; crush.
+    cbn.
+
+    (* application works *)
+    eapply valrel_in_termrel in vr₁'.
+    eapply (termrel_app vr₁').
+
+    (* application argument is also fine *)
+    eauto using valrel_in_termrel, valrel_mono.
+  - (* unk case *) 
+    eapply dwp_imprecise in dwp; subst.
+    eapply termrel_div_lt.
+    fold (caseArr n vs₁').
+    eapply (divergence_closed_under_evalcontext' div); S.inferContext; crush.
+  - (* other cases *)
+    
+    eapply termrel_div_wrong.
+    + fold (caseArr n vs₁').
+      eapply (divergence_closed_under_evalcontext' div); S.inferContext; crush.
+    + right.
+      eapply evalToStar.
+      eapply U.eval₀_to_eval.
+      eauto with eval.
+Qed.
+
+
+Lemma compat_emul_app {n m d p Γ ts₁ tu₁ ts₂ tu₂} :
+  dir_world_prec n m d p →
+  ⟪ Γ ⊩ ts₁ ⟦ d , m ⟧ tu₁ : pEmulDV n p ⟫ →
+  ⟪ Γ ⊩ ts₂ ⟦ d , m ⟧ tu₂ : pEmulDV n p ⟫ →
+  ⟪ Γ ⊩ S.app (S.app (S.abs (UVal n) (S.abs (UVal n) (S.app (caseArrUp n (S.var 1)) (S.var 0)))) ts₁) ts₂ ⟦ d , m ⟧ U.app tu₁ tu₂ : pEmulDV n p ⟫.
+Proof.
+  intros dwp [ty₁ tr₁] [ty₂ tr₂].
+  split.
+  - eauto using caseArrUp_T with typing uval_typing.
+  - intros w wn γs γu envrel.
+    unfold lev in *.
+
+    specialize (tr₁ w wn γs γu envrel).
+    assert (dir_world_prec n w d p) by eauto using dwp_mono.
+
+    change (S.app (caseArrUp n ts₁) ts₂)[γs] 
+    with (S.app (caseArrUp n ts₁) [γs] ts₂[γs]).
+    change (U.app tu₁ tu₂)[γu] with (U.app tu₁[γu] tu₂[γu]).
+    cbn; crush.
+    rewrite caseArrUp_sub; cbn; crush.
+    change (wk 0) with 1.
+
+    eapply termrel_caseArrUp; eauto.
+    intros w' futw.
+    eauto using envrel_mono with arith.
+Qed.
